Add option to fmap node values.
The option type has several advantages that I think will provide a
better overall performance: inserts are cheap (because node values
can be left empty), composing is cheaper (because at identity
mappings we can directly graft the value from g), inverting is
cheaper (because we only insert inverse mappings at non-identity
nodes).

I am unsure about the performance benefit of explicit pruning. No
pruning will diminish the above benefits over the course of
compositions, but pruning is also expensive. I have changed the
definition of pruning into a more general sifting procedure that
removes mappings already present in a given tree. It might make
sense to periodically apply this to permutations.

B1_fmap.v
@@ -5,167 +5,223 @@ From permutation_solver Require Import A_setup.
 Open Scope positive.
 
 (***
-We start with some utilities for positive numbers.
+Operations on positive numbers
 *)
 
+(* Reverse append i to an accumulator. *)
+Fixpoint lifo (i acc : positive) :=
+  match i with
+  | xH => acc
+  | xO i' => lifo i' (xO acc)
+  | xI i' => lifo i' (xI acc)
+  end.
+
+Notation mirror i := (lifo i xH).
+
 (***
+Unbalanced binary tree
+
 Using an unbalanced tree has several interesting advantages:
 - Implementation is simpler.
 - Creation does not require balancing.
 - Lookup does not require key comparison.
 *)
 
-Inductive fmap := Ident | Node (i : positive) (f0 f1 : fmap).
+Inductive fmap := Leaf | Node (iO : option positive) (f0 f1 : fmap).
 
-(* Get the submap under a given branch. *)
-Fixpoint truncate (f : fmap) (i : positive) :=
+(***
+Insert and lookup mappings
+*)
+
+(* Insert j at i. *)
+Fixpoint insert (f : fmap) (i j : positive) :=
   match f with
-  | Ident => Ident
-  | Node j f0 f1 =>
+  | Leaf =>
     match i with
-    | xH => f
-    | xO i' => truncate f0 i'
-    | xI i' => truncate f1 i'
+    | xH => Node (Some j) Leaf Leaf
+    | xO i' => Node None (insert Leaf i' j) Leaf
+    | xI i' => Node None Leaf (insert Leaf i' j)
+    end
+  | Node iO f0 f1 =>
+    match i with
+    | xH => Node (Some j) f0 f1
+    | xO i' => Node iO (insert f0 i' j) f1
+    | xI i' => Node iO f0 (insert f1 i' j)
     end
   end.
 
-(* Apply f to i. The input index must be repeated for the Ident case. *)
-Fixpoint apply (f : fmap) (i : positive) : positive -> positive :=
+(* Get the value at i. *)
+Fixpoint lookup (f : fmap) (i : positive) : option positive :=
   match f with
-  | Ident => λ j, j
-  | Node j f0 f1 =>
+  | Leaf => None
+  | Node jO f0 f1 =>
     match i with
-    | xH => λ _, j
-    | xO i' => apply f0 i'
-    | xI i' => apply f1 i'
+    | xH => jO
+    | xO i' => lookup f0 i'
+    | xI i' => lookup f1 i'
     end
   end.
 
-Notation "f ⋅ i" := (apply f i i) (at level 5, format "f ⋅ i").
+(***
+Function application
+*)
+
+Definition apply f i :=
+  match lookup f i with
+  | Some j => j
+  | None => i
+  end.
+
+Notation "f ⋅ i" := (apply f i) (at level 5, format "f ⋅ i").
+
+(***
+Function composition
+*)
+
+(* Apply g to all mappings in f. *)
+Fixpoint fmap_map (g f : fmap) :=
+  match f with
+  | Leaf => Leaf
+  | Node (Some i) f0 f1 => Node (Some g⋅i) (fmap_map g f0) (fmap_map g f1)
+  | Node None f0 f1 => Node None (fmap_map g f0) (fmap_map g f1)
+  end.
 
 (* Apply g after f. The initial input for g must be copied as gI. *)
 Fixpoint compose (gI g f : fmap) {struct f} :=
   match f with
-  | Ident => g
-  | Node j f0 f1 =>
+  | Leaf => g
+  | Node (Some i) f0 f1 =>
     match g with
-    | Ident => Node (gI⋅j) (compose gI Ident f0) (compose gI Ident f1)
-    | Node _ g0 g1 => Node (gI⋅j) (compose gI g0 f0) (compose gI g1 f1)
+    | Leaf => Node (Some gI⋅i) (fmap_map gI f0) (fmap_map gI f1)
+    | Node jO g0 g1 => Node (Some gI⋅i) (compose gI g0 f0) (compose gI g1 f1)
+    end
+  | Node None f0 f1 =>
+    match g with
+    | Leaf => Node None (fmap_map gI f0) (fmap_map gI f1)
+    | Node jO g0 g1 => Node jO (compose gI g0 f0) (compose gI g1 f1)
     end
   end.
 
-(* Reverse a positive number (path to index) andd add to accumulator. *)
-Fixpoint revp (r acc : positive) :=
-  match r with
-  | xH => acc
-  | xO r' => revp r' (xO acc)
-  | xI r' => revp r' (xI acc)
-  end.
+Notation "g ∘ f" := (compose g g f) (at level 50).
 
-(* Prune identity branches give we are at branch r. *)
-Fixpoint prune (f : fmap) (r : positive) :=
+(***
+Function inversion
+*)
+
+(* Invert a surjective map. *)
+Fixpoint invert (f f_inv : fmap) (r : positive) :=
   match f with
-  | Ident => Ident
-  | Node j f0 f1 =>
-    match prune f0 (xO r), prune f1 (xI r) with
-    | Ident, Ident => if revp r xH =? j then Ident else Node j Ident Ident
-    | f0', f1' => Node j f0' f1'
+  | Leaf => f_inv
+  | Node iO f0 f1 =>
+    let f_inv' := invert f0 f_inv r~0 in
+    let f_inv'' := invert f1 f_inv' r~1 in
+    match iO with
+    | Some i => insert f_inv'' i (mirror r)
+    | None => f_inv''
     end
   end.
 
-Notation "g ∘ f" := (prune (compose g g f) xH) (at level 50).
+Notation inv f := (invert f Leaf xH).
 
 (***
-Lets state some boring, obvious results.
+Pruning
+
+There are several advantages of pruning (removing identity mappings) trees after
+composition. There is a slight advantage for lookups, but more importantly;
+compositions will be faster. The inversion function we define later will also
+benefit from pruning. But, this optimization is more tricky than it seems,
+because pruning is quite expensive. We have to compare every mapping to its key
+path, and, when recursively iterating the tree, we have to keep track of the
+position of every node which requires appending bits to the end of a `positive`.
+
+Because we will be working with permutations on the same finite domain, I think
+this pruning procedure can be optimized a little by pre-computing the tree of
+all identity mappings. Hence I have implemented a sifting function that removes
+the mappings that are present in a given tree. We will have to determine in
+practice if this sifting procedure actually provides a net speed-up.
 *)
 
-Lemma fmap_eq_dec (f g : fmap) :
-  {f = g} + {f ≠ g}.
-Proof.
-revert g; induction f as [|j f0 Hf0 f1 Hf1]; intros [].
-now left. 1,2: now right.
-destruct (Pos.eq_dec j i); subst.
-destruct (Hf0 f2); subst.
-destruct (Hf1 f3); subst.
-now left. all: right; congruence.
-Qed.
+(* A pruned fmap contains no explicit identity mappings. *)
+Fixpoint Pruned (f : fmap) (r : positive) :=
+  match f with
+  | Leaf => True
+  | Node iO f0 f1 =>
+    Pruned f0 r~0 /\
+    Pruned f1 r~1 /\
+    match iO with
+    | Some i => i ≠ mirror r
+    | None => True
+    end
+  end.
+
+(* Remove the mappings in f that are also in s. *)
+Fixpoint sift (f s : fmap) :=
+  let collapse := λ (f0 f1 : fmap),
+    match f0, f1 with
+    | Leaf, Leaf => Leaf
+    | f0', f1' => Node None f0' f1'
+    end
+  in match s with
+  | Leaf => f
+  | Node iO s0 s1 =>
+    match f with
+    | Leaf => Leaf
+    | Node None f0 f1 => collapse (sift f0 s0) (sift f1 s1)
+    | Node (Some j) f0 f1 =>
+      match iO with
+      | Some i =>
+        if i =? j
+        then collapse (sift f0 s0) (sift f1 s1)
+        else Node (Some j) (sift f0 s0) (sift f1 s1)
+      | None => Node (Some j) (sift f0 s0) (sift f1 s1)
+      end
+    end
+  end.
 
 (***
-We now want to prove that composition and pruning agree with application.
+Theorems
 *)
 
-Lemma revp_shift_xO r i : revp r i~0 = revp r~0 i.
-Proof. easy. Qed.
+Local Ltac fmap_induction f :=
+  induction f as [|jO f0 IHf0 f1 IHf1]; simpl; intros.
 
-Lemma revp_shift_xI r i : revp r i~1 = revp r~1 i.
-Proof. easy. Qed.
-
-(* Pruning does not alter the mapping. *)
-Theorem prune_apply f r i :
-  apply (prune f r) i (revp r i) = apply f i (revp r i).
+Lemma lookup_fmap_map_None g f i :
+  lookup f i = None -> lookup (fmap_map g f) i = None.
 Proof.
-revert r i; induction f as [|j f0 IHf0 f1 IHf1]; intros. easy.
-simpl prune. destruct (prune f0 _) eqn:H0. destruct (prune f1 _) eqn:H1.
-(* The second and third goal are actually exactly the same. *)
-2: rewrite <-H0, <-H1; clear H0 H1. 3: rewrite <-H0; clear H0.
-(* First solve the double Ident case. *)
-{ destruct (revp r 1 =? j) eqn:E; simpl; destruct i.
-  2,5: rewrite revp_shift_xO, <-IHf0, H0; easy.
-  1,3: rewrite revp_shift_xI, <-IHf1, H1; easy.
-  apply Pos.eqb_eq, E. reflexivity. }
-(* Solve the remaining goals simultaneously.*)
-all: simpl; destruct i; try reflexivity.
-2,4: rewrite revp_shift_xO, <-IHf0; easy.
-1,2: rewrite revp_shift_xI, <-IHf1; easy.
+revert i; fmap_induction f. easy.
+destruct i, jO as [j|]; simpl; try easy.
+all: try apply IHf0; try apply IHf1; easy.
 Qed.
 
-Corollary prune_xH_apply f i :
-  (prune f xH)⋅i = f⋅i.
+Lemma lookup_compose_None gI g f i :
+  lookup f i = None -> lookup (compose gI g f) i = lookup g i.
 Proof.
-apply prune_apply.
+revert g i; fmap_induction f. easy.
+destruct jO as [j|], g, i; simpl; try easy.
+1,2,5,6: apply lookup_fmap_map_None, H.
+all: try rewrite IHf1; try rewrite IHf0; easy.
 Qed.
 
-(* If f is Ident at i, then f⋅i = i. *)
-Lemma truncate_Ident_apply f i iI :
-  truncate f i = Ident -> apply f i iI = iI.
+Lemma lookup_fmap_map_Some g f i j :
+  lookup f i = Some j -> lookup (fmap_map g f) i = Some g⋅j.
 Proof.
-revert i; induction f as [|j f0 IHf0 f1 IHf1]; simpl; intros. easy.
-destruct i. apply IHf1, H. apply IHf0, H. discriminate H.
+revert g i; fmap_induction f. easy.
+destruct jO as [j'|], i; simpl; try congruence.
+all: try apply IHf0; try apply IHf1; easy.
 Qed.
 
-(* If f is the identity at i, then the sub-branch of g is used. *)
-Lemma compose_apply_Ident gI g f i iI :
-  truncate f i = Ident -> apply (compose gI g f) i iI = apply g i iI.
+Lemma lookup_compose_Some gI g f i j :
+  lookup f i = Some j -> lookup (compose gI g f) i = Some gI⋅j.
 Proof.
-revert g i iI; induction f as [|j f0 IHf0 f1 IHf1]; simpl; intros. easy.
-destruct i, g; simpl; try discriminate H.
-rewrite IHf1; easy. apply IHf1, H.
-rewrite IHf0; easy. apply IHf0, H.
+revert g i; induction f as [|jO f0 IHf0 f1 IHf1]; simpl; intros. easy.
+destruct jO as [j'|], g, i; simpl; try congruence.
+all: try apply lookup_fmap_map_Some; try apply IHf0; try apply IHf1; easy.
 Qed.
 
-(* If f is not the identity at i, then gI is applied to the node value. *)
-Lemma compose_apply_not_Ident gI g f i iI :
-  truncate f i ≠ Ident -> apply (compose gI g f) i iI = gI⋅(apply f i iI).
-Proof.
-revert g i iI; induction f as [|j f0 IHf0 f1 IHf1]; intros. easy.
-destruct g, i; simpl in *; try reflexivity.
-2,4: apply IHf0, H. 1,2: apply IHf1, H.
-Qed.
-
-Theorem compose_apply g f i :
-  (compose g g f)⋅i = g⋅(f⋅i).
-Proof.
-(* We split into two cases based on `truncate f i`. *)
-destruct (truncate f i) eqn:H.
-- eapply truncate_Ident_apply in H as Hf; rewrite Hf.
-  apply compose_apply_Ident, H.
-- apply compose_apply_not_Ident; congruence.
-Qed.
-
-Corollary comp_apply g f i :
+Corollary apply_compose g f i :
   (g ∘ f)⋅i = g⋅(f⋅i).
 Proof.
-etransitivity.
-apply prune_apply.
-apply compose_apply.
+unfold apply; destruct (lookup f i) as [j|] eqn:H.
+erewrite lookup_compose_Some; easy.
+erewrite lookup_compose_None; easy.
 Qed.
